Quick refactoring of Typ and PTyp into Sort

theories/autosubst/AST.sig
@@ -1,12 +1,12 @@
 -- Universe levels
 level : Type
+sort : Type
 
 -- Syntax
 
 term(var) : Type
 
-Typ : level -> term
-PTyp : level -> term
+Sort : sort -> level -> term
 
 Pi : term -> (bind term in term) -> term
 lam : term -> (bind term in term) -> term
